Make pure_to_thunk smarter regarding Delay

compiler/backend/passes/proofs/pure_to_thunk_2ProofScript.sml
@@ -8,6 +8,7 @@ open stringTheory optionTheory sumTheory pairTheory listTheory alistTheory
      pure_semanticsTheory thunkLangTheory thunk_semanticsTheory pure_evalTheory
      thunkLang_primitivesTheory pure_exp_lemmasTheory pure_miscTheory
      pure_to_thunk_1ProofTheory pure_cexpTheory pureLangTheory
+     thunk_unthunkProofTheory
      thunk_case_liftProofTheory
      thunk_case_projProofTheory thunk_exp_ofTheory
      thunk_let_forceProofTheory
@@ -30,9 +31,11 @@ Inductive exp_rel:
      exp_rel x y ⇒
        exp_rel (pure_cexp$Lam i s x) (Lam s y)) ∧
 [~Let:]
-  (∀s x y x1 y1.
-     exp_rel x x1 ∧ exp_rel y y1 ⇒
-       exp_rel (Let i s x y) (Let (SOME s) (Delay x1) y1)) ∧
+  (∀s x y z1 y1.
+     (~(∃c v. x = Var c v ∧ z1 = Var v) ⇒
+      (∃x1. exp_rel x x1 ∧ z1 = Delay x1)) ∧
+     exp_rel y y1 ⇒
+       exp_rel (Let i s x y) (Let (SOME s) z1 y1)) ∧
 [~Letrec:]
   (∀i xs xs1 y y1.
      LIST_REL (λ(n,x) (m,x1). n = m ∧
@@ -41,12 +44,14 @@ Inductive exp_rel:
 [~App:]
   (∀f g xs ys.
      exp_rel f g ∧
-     LIST_REL exp_rel xs ys ⇒
-       exp_rel (App i f xs) (App g (MAP Delay ys))) ∧
+     LIST_REL (λx z1. ~(∃c v. x = Var c v ∧ z1 = Var v) ⇒
+                      (∃x1. exp_rel x x1 ∧ z1 = Delay x1)) xs ys ⇒
+       exp_rel (App i f xs) (App g ys)) ∧
 [~Cons:]
   (∀xs ys n.
-     LIST_REL exp_rel xs ys ⇒
-       exp_rel (Prim i (Cons n) xs) (Prim (Cons n) (MAP Delay ys))) ∧
+     LIST_REL (λx z1. ~(∃c v. x = Var c v ∧ z1 = Var v) ⇒
+                      (∃x1. exp_rel x x1 ∧ z1 = Delay x1)) xs ys ⇒
+       exp_rel (Prim i (Cons n) xs) (Prim (Cons n) ys)) ∧
 [~Prim:]
   (∀xs ys a.
      LIST_REL exp_rel xs ys ⇒
@@ -63,10 +68,12 @@ Inductive exp_rel:
        x1 = y1 ∧ x2 = y2 ∧ ~MEM fresh x2 ∧
        exp_rel x3 y3 ∧ explode fresh ∉ freevars (exp_of' x3)) xs ys ∧
      (∀a x. eopt = SOME (a,x) ⇒ explode fresh ∉ freevars (exp_of' x)) ∧
-     exp_rel x a_exp ∧ fresh ≠ v ∧
+     (~(∃c z. x = Var c z ∧ a_exp = Var z) ⇒
+      (∃x1. exp_rel x x1 ∧ a_exp = Delay x1)) ∧
+     fresh ≠ v ∧
      OPTREL (λ(a,x) (b,y). a = b ∧ exp_rel x y) eopt yopt ⇒
        exp_rel (Case i x v xs eopt)
-               (Let (SOME v) (Delay a_exp) $
+               (Let (SOME v) a_exp $
                 Let (SOME fresh) (Force (Var v)) $
                   Case fresh ys yopt))
 End
@@ -75,6 +82,7 @@ Overload to_thunk = “pure_to_thunk_1Proof$compile_rel”
 Overload lift_rel = “thunk_case_liftProof$compile_rel”
 Overload force_rel = “thunk_let_forceProof$exp_rel”
 Overload proj_rel = “thunk_case_projProof$compile_rel”
+Overload delay_force = “thunk_unthunkProof$delay_force”
 
 Overload VV[local] = “thunk_let_forceProof$Var”
 
@@ -85,16 +93,18 @@ Theorem lets_for_lemma[local]:
     to_thunk (exp_of' h2) y1 ∧
     lift_rel y1 y2 ∧
     force_rel NONE y2 y3 ∧
-    proj_rel y3 (exp_of yy2) ∧
+    proj_rel y3 y4 ∧
+    delay_force y4 (exp_of yy2) ∧
     ~MEM fresh vs ∧ ~MEM h vs ∧ fresh ≠ h ∧
     fresh ∉ freevars (exp_of' h2) ⇒
-    ∃x1 x2 x3.
+    ∃x1 x2 x3 x4.
       to_thunk
         (lets_for' (k + LENGTH vs) cn h
           (MAPi (λx v. (x+k,v)) vs) (exp_of' h2)) x1 ∧
       lift_rel x1 x2 ∧ fresh ∉ freevars x1 ∧
       force_rel (SOME (VV h,fresh)) x2 x3 ∧
-      proj_rel x3
+      proj_rel x3 x4 ∧
+      delay_force x4
         (lets_for (k + LENGTH vs) cn fresh
           (MAPi (λx v. (x+k,v)) vs) (exp_of yy2))
 Proof
@@ -132,6 +142,15 @@ Proof
   \\ irule_at Any thunk_case_liftProofTheory.compile_rel_Prim \\ fs [PULL_EXISTS]
   \\ irule_at Any thunk_case_liftProofTheory.compile_rel_Force
   \\ irule_at Any thunk_case_liftProofTheory.compile_rel_Var
+  \\ irule_at Any thunk_unthunkProofTheory.delay_force_Let
+  \\ irule_at Any thunk_unthunkProofTheory.delay_force_If \\ fs []
+  \\ irule_at Any thunk_unthunkProofTheory.delay_force_Prim \\ fs []
+  \\ irule_at Any thunk_unthunkProofTheory.delay_force_Prim \\ fs []
+  \\ irule_at Any thunk_unthunkProofTheory.delay_force_Var \\ fs []
+  \\ irule_at Any thunk_unthunkProofTheory.delay_force_Prim \\ fs []
+  \\ irule_at Any thunk_unthunkProofTheory.delay_force_Let
+  \\ irule_at Any thunk_unthunkProofTheory.delay_force_Prim \\ fs []
+  \\ irule_at Any thunk_unthunkProofTheory.delay_force_Var \\ fs []
   \\ rpt $ first_x_assum $ irule_at Any
   \\ irule_at Any thunk_let_forceProofTheory.exp_rel_Let
   \\ fs [name_clash_def]
@@ -184,6 +203,15 @@ Proof
   \\ rpt (irule_at Any thunk_case_projProofTheory.compile_rel_Var \\ fs [])
 QED
 
+Theorem delay_force_Disj:
+  ∀xs v. delay_force (Disj v xs) (Disj v xs)
+Proof
+  Induct \\ fs [Disj_def,FORALL_PROD] \\ rw []
+  \\ rpt (irule_at Any thunk_unthunkProofTheory.delay_force_If \\ fs [])
+  \\ rpt (irule_at Any thunk_unthunkProofTheory.delay_force_Prim \\ fs [])
+  \\ rpt (irule_at Any thunk_unthunkProofTheory.delay_force_Var \\ fs [])
+QED
+
 Triviality freevars_Disj':
   ∀xs. f ≠ v ⇒ f ∉ freevars (Disj' (Force (Var v)) xs)
 Proof
@@ -194,16 +222,19 @@ QED
 Theorem exp_rel_imp_combined:
   ∀x y.
     exp_rel x y ∧ cexp_wf x ⇒
-    ∃y1 y2 y3.
+    ∃y1 y2 y3 y4.
       to_thunk (exp_of' x) y1 ∧
       lift_rel y1 y2 ∧
       force_rel NONE y2 y3 ∧
-      proj_rel y3 (exp_of y)
+      proj_rel y3 y4 ∧
+      delay_force y4 (exp_of y)
 Proof
   Induct_on ‘exp_rel’
   \\ rw [exp_of'_def,pure_cexpTheory.cexp_wf_def] \\ fs [pure_cexpTheory.op_of_def]
   >~ [‘Var n’] >-
    (simp [Once pure_to_thunk_1ProofTheory.compile_rel_cases]
+    \\ irule_at Any thunk_unthunkProofTheory.delay_force_Force
+    \\ irule_at Any thunk_unthunkProofTheory.delay_force_Var
     \\ irule_at Any thunk_case_liftProofTheory.compile_rel_Force
     \\ irule_at Any thunk_case_liftProofTheory.compile_rel_Var
     \\ irule_at Any thunk_let_forceProofTheory.exp_rel_Force
@@ -215,14 +246,39 @@ Proof
     \\ irule_at Any thunk_let_forceProofTheory.exp_rel_Let
     \\ irule_at Any thunk_case_liftProofTheory.compile_rel_Let
     \\ fs [name_clash_def]
+    \\ irule_at Any thunk_unthunkProofTheory.delay_force_Let
     \\ simp [Once pure_to_thunk_1ProofTheory.compile_rel_cases,PULL_EXISTS]
+    \\ irule_at Any thunk_unthunkProofTheory.delay_force_Let
+    \\ irule_at Any thunk_unthunkProofTheory.delay_force_Force
+    \\ irule_at Any thunk_unthunkProofTheory.delay_force_Var
     \\ irule_at Any thunk_case_liftProofTheory.compile_rel_Delay
     \\ irule_at Any thunk_let_forceProofTheory.exp_rel_Delay
     \\ irule_at Any thunk_case_projProofTheory.compile_rel_Delay
-    \\ qpat_x_assum ‘proj_rel y3 (exp_of y)’ $ irule_at Any
-    \\ qpat_x_assum ‘force_rel NONE y2 y3’ $ irule_at Any
-    \\ qpat_x_assum ‘lift_rel y1 y2’ $ irule_at Any
-    \\ qpat_x_assum ‘to_thunk (exp_of' x) y1’ $ irule_at Any
+    \\ gvs [PULL_EXISTS]
+    \\ ‘∃q1 q2 q3 q4.
+          to_thunk (exp_of' x) q1 ∧
+          lift_rel q1 q2 ∧
+          force_rel NONE q2 q3 ∧
+          proj_rel q3 q4 ∧
+          delay_force (Delay q4) (exp_of a_exp)’ by
+      (qpat_x_assum ‘(∀c z. x = Var c z ⇒ a_exp ≠ Var z) ⇒ _’ mp_tac
+       \\ disch_then (assume_tac o ONCE_REWRITE_RULE [IMP_DISJ_THM])
+       \\ reverse $ gvs []
+       >- metis_tac [delay_force_Delay]
+       \\ fs [exp_of'_def]
+       \\irule_at Any pure_to_thunk_1ProofTheory.compile_rel_Var
+       \\ irule_at Any thunk_case_liftProofTheory.compile_rel_Force
+       \\ irule_at Any thunk_let_forceProofTheory.exp_rel_Force
+       \\ irule_at Any thunk_case_projProofTheory.compile_rel_Force
+       \\ irule_at Any thunk_case_liftProofTheory.compile_rel_Var
+       \\ irule_at Any thunk_let_forceProofTheory.exp_rel_Var
+       \\ irule_at Any thunk_case_projProofTheory.compile_rel_Var
+       \\ irule_at Any thunk_unthunkProofTheory.delay_force_Delat_Force_Var)
+    \\ qpat_x_assum ‘to_thunk (exp_of' x) _’ $ irule_at Any
+    \\ qpat_x_assum ‘lift_rel _ _’ $ irule_at Any
+    \\ qpat_x_assum ‘force_rel NONE _ _’ $ irule_at Any
+    \\ qpat_x_assum ‘proj_rel _ _’ $ irule_at Any \\ fs []
+    \\ qpat_x_assum ‘(∀c z. x = Var c z ⇒ a_exp ≠ Var z) ⇒ _’ kall_tac
     \\ Cases_on ‘xs’ \\ fs []
     \\ PairCases_on ‘h’ \\ fs []
     \\ rename [‘_ = yy :: _’]
@@ -246,6 +302,9 @@ Proof
     \\ irule_at Any thunk_case_projProofTheory.compile_rel_If \\ fs []
     \\ irule_at Any thunk_case_projProofTheory.compile_rel_Prim \\ fs []
     \\ irule_at Any thunk_case_projProofTheory.compile_rel_Var \\ fs []
+    \\ irule_at Any thunk_unthunkProofTheory.delay_force_If \\ fs []
+    \\ irule_at Any thunk_unthunkProofTheory.delay_force_Prim \\ fs []
+    \\ irule_at Any thunk_unthunkProofTheory.delay_force_Var \\ fs []
     \\ drule lets_for_lemma
     \\ rpt $ disch_then drule
     \\ ‘¬MEM (explode fresh) (MAP explode h1)’ by fs [MEM_EQ_MEM_MAP_explode]
@@ -267,12 +326,14 @@ Proof
       \\ Cases_on ‘yopt’ \\ fs []
       \\ Cases_on ‘eopt’ \\ gvs []
       >-
-       (irule_at Any thunk_case_projProofTheory.compile_rel_Prim \\ fs []
+       (irule_at Any thunk_unthunkProofTheory.delay_force_Prim \\ fs []
+        \\ irule_at Any thunk_case_projProofTheory.compile_rel_Prim \\ fs []
         \\ irule_at Any thunk_let_forceProofTheory.exp_rel_Prim \\ fs []
         \\ irule_at Any thunk_case_liftProofTheory.compile_rel_Prim \\ fs []
         \\ simp [Once pure_to_thunk_1ProofTheory.compile_rel_cases, freevars_def])
       \\ PairCases_on ‘x'’ \\ PairCases_on ‘x''’ \\ gvs []
       \\ fs [IfDisj_def]
+      \\ irule_at Any thunk_unthunkProofTheory.delay_force_If \\ fs []
       \\ irule_at Any thunk_case_projProofTheory.compile_rel_If \\ fs []
       \\ irule_at Any thunk_let_forceProofTheory.exp_rel_If \\ fs []
       \\ irule_at Any thunk_case_liftProofTheory.compile_rel_If \\ fs []
@@ -289,9 +350,12 @@ Proof
       \\ irule_at Any thunk_let_forceProofTheory.exp_rel_Prim \\ fs []
       \\ irule_at Any proj_rel_Disj
       \\ fs [freevars_def,SF DNF_ss]
+      \\ first_assum $ irule_at $ Pos hd
       \\ fs [] \\ imp_res_tac to_thunk_freevars \\ fs []
       \\ irule_at Any thunk_case_projProofTheory.compile_rel_Prim \\ fs []
-      \\ irule freevars_Disj' \\ fs [])
+      \\ irule_at Any freevars_Disj' \\ fs []
+      \\ irule_at Any thunk_unthunkProofTheory.delay_force_Prim \\ fs []
+      \\ irule_at Any delay_force_Disj)
     \\ fs [FORALL_PROD]
     \\ rw [] \\ gvs []
     \\ first_x_assum dxrule
@@ -306,6 +370,9 @@ Proof
     \\ irule_at Any thunk_case_liftProofTheory.compile_rel_Prim \\ fs [PULL_EXISTS]
     \\ irule_at Any thunk_case_liftProofTheory.compile_rel_Force
     \\ irule_at Any thunk_case_liftProofTheory.compile_rel_Var
+    \\ irule_at Any thunk_unthunkProofTheory.delay_force_If \\ fs [PULL_EXISTS]
+    \\ irule_at Any thunk_unthunkProofTheory.delay_force_Prim \\ fs [PULL_EXISTS]
+    \\ irule_at Any thunk_unthunkProofTheory.delay_force_Var
     \\ irule_at Any thunk_case_projProofTheory.compile_rel_If \\ fs [PULL_EXISTS]
     \\ irule_at Any thunk_case_projProofTheory.compile_rel_Prim \\ fs [PULL_EXISTS]
     \\ irule_at Any thunk_case_projProofTheory.compile_rel_Var
@@ -313,7 +380,7 @@ Proof
     \\ simp [Once thunk_let_forceProofTheory.exp_rel_cases]
     \\ simp [Once thunk_let_forceProofTheory.exp_rel_cases]
     \\ drule lets_for_lemma
-    \\ ntac 3 $ disch_then drule
+    \\ ntac 4 $ disch_then drule
     \\ disch_then $ drule_at $ Pos last
     \\ rename [‘lets_for' (LENGTH cs) (explode cn)’]
     \\ disch_then $ qspecl_then [‘explode v’,
@@ -322,7 +389,8 @@ Proof
     \\ fs [] \\ strip_tac
     \\ rpt $ pop_assum $ irule_at Any
     \\ first_assum $ irule_at Any
-    \\ first_assum $ irule_at Any)
+    \\ first_assum $ irule_at Any
+    \\ fs [])
   >~ [‘Seq’] >-
    (fs [pure_cexpTheory.op_of_def]
     \\ irule_at Any pure_to_thunk_1ProofTheory.compile_rel_Seq_fresh \\ fs []
@@ -331,22 +399,38 @@ Proof
     \\ irule_at Any thunk_let_forceProofTheory.exp_rel_Let
     \\ fs [name_clash_def]
     \\ irule_at Any thunk_case_projProofTheory.compile_rel_Let_SOME
+    \\ irule_at Any thunk_unthunkProofTheory.delay_force_Let
     \\ metis_tac [])
   >~ [‘Let’] >-
    (irule_at Any pure_to_thunk_1ProofTheory.compile_rel_Let
     \\ irule_at Any thunk_case_liftProofTheory.compile_rel_Let
-    \\ irule_at Any thunk_case_liftProofTheory.compile_rel_Delay
     \\ irule_at Any thunk_let_forceProofTheory.exp_rel_Let
-    \\ irule_at Any thunk_let_forceProofTheory.exp_rel_Delay
     \\ fs [name_clash_def]
     \\ irule_at Any thunk_case_projProofTheory.compile_rel_Let_SOME
+    \\ irule_at Any thunk_unthunkProofTheory.delay_force_Let
+    \\ irule_at Any thunk_case_liftProofTheory.compile_rel_Delay
+    \\ irule_at Any thunk_let_forceProofTheory.exp_rel_Delay
     \\ irule_at Any thunk_case_projProofTheory.compile_rel_Delay
+    \\ gvs [IMP_DISJ_THM,exp_of'_def]
+    >-
+     (irule_at Any pure_to_thunk_1ProofTheory.compile_rel_Var
+      \\ irule_at Any thunk_case_liftProofTheory.compile_rel_Force
+      \\ irule_at Any thunk_let_forceProofTheory.exp_rel_Force
+      \\ irule_at Any thunk_case_projProofTheory.compile_rel_Force
+      \\ irule_at Any thunk_case_liftProofTheory.compile_rel_Var
+      \\ irule_at Any thunk_let_forceProofTheory.exp_rel_Var
+      \\ irule_at Any thunk_case_projProofTheory.compile_rel_Var
+      \\ irule_at Any thunk_unthunkProofTheory.delay_force_Delat_Force_Var
+      \\ metis_tac [])
+    \\ irule_at Any thunk_unthunkProofTheory.delay_force_Delay
     \\ metis_tac [])
   >~ [‘Cons _ _’] >-
    (irule_at Any pure_to_thunk_1ProofTheory.compile_rel_Cons
     \\ irule_at Any thunk_case_liftProofTheory.compile_rel_Prim
     \\ irule_at Any thunk_let_forceProofTheory.exp_rel_Prim
     \\ irule_at Any thunk_case_projProofTheory.compile_rel_Cons
+    \\ irule_at Any thunk_unthunkProofTheory.delay_force_Prim
+    \\ fs []
     \\ pop_assum mp_tac
     \\ pop_assum kall_tac
     \\ pop_assum mp_tac
@@ -354,12 +438,37 @@ Proof
     \\ qid_spec_tac ‘xs’
     \\ Induct \\ fs [PULL_EXISTS]
     \\ rw [] \\ gvs []
-    \\ irule_at Any thunk_case_projProofTheory.compile_rel_Delay
-    \\ irule_at Any thunk_let_forceProofTheory.exp_rel_Delay
-    \\ irule_at Any thunk_case_liftProofTheory.compile_rel_Delay
+    \\ fs [thunk_unthunkProofTheory.is_delay_def]
     \\ rpt $ first_assum $ irule_at Any
     \\ last_x_assum drule \\ strip_tac
-    \\ rpt $ first_assum $ irule_at Any)
+    \\ rpt $ first_assum $ irule_at Any
+    \\ rpt $ qpat_x_assum ‘LIST_REL _ _ _’ kall_tac
+    \\ qpat_x_assum ‘(∀c z. h = Var c z ⇒ h5 ≠ Var z) ⇒ _’ mp_tac
+    \\ disch_then (assume_tac o ONCE_REWRITE_RULE [IMP_DISJ_THM])
+    \\ reverse $ gvs []
+    >-
+     (qpat_x_assum ‘to_thunk (exp_of' _) _’ $ irule_at Any
+      \\ irule_at Any thunk_case_liftProofTheory.compile_rel_Delay
+      \\ qpat_x_assum ‘lift_rel y1 _’ $ irule_at Any
+      \\ irule_at Any thunk_let_forceProofTheory.exp_rel_Delay
+      \\ qpat_x_assum ‘force_rel NONE y2 _’ $ irule_at Any
+      \\ irule_at Any thunk_case_projProofTheory.compile_rel_Delay
+      \\ first_x_assum $ irule_at $ Pos hd
+      \\ fs [thunk_unthunkProofTheory.is_delay_def]
+      \\ irule_at Any thunk_unthunkProofTheory.delay_force_Delay \\ fs [])
+    \\ fs [cexp_wf_def,SF SFY_ss,exp_of'_def]
+    \\ irule_at Any pure_to_thunk_1ProofTheory.compile_rel_Var
+    \\ irule_at Any thunk_case_liftProofTheory.compile_rel_Delay
+    \\ irule_at Any thunk_case_liftProofTheory.compile_rel_Force
+    \\ irule_at Any thunk_case_liftProofTheory.compile_rel_Var
+    \\ irule_at Any thunk_let_forceProofTheory.exp_rel_Delay
+    \\ irule_at Any thunk_let_forceProofTheory.exp_rel_Force
+    \\ irule_at Any thunk_let_forceProofTheory.exp_rel_Var
+    \\ irule_at Any thunk_case_projProofTheory.compile_rel_Delay
+    \\ irule_at Any thunk_case_projProofTheory.compile_rel_Force
+    \\ irule_at Any thunk_case_projProofTheory.compile_rel_Var
+    \\ irule_at Any thunk_unthunkProofTheory.delay_force_Delat_Force_Var
+    \\ fs [thunk_unthunkProofTheory.is_delay_def])
   >~ [‘Apps’] >-
    (pop_assum kall_tac
     \\ rpt $ pop_assum mp_tac
@@ -367,6 +476,7 @@ Proof
     \\ qid_spec_tac ‘y1’
     \\ qid_spec_tac ‘y2’
     \\ qid_spec_tac ‘y3’
+    \\ qid_spec_tac ‘y4’
     \\ qid_spec_tac ‘y’
     \\ qid_spec_tac ‘ys’
     \\ qid_spec_tac ‘xs’
@@ -374,12 +484,12 @@ Proof
     >- (fs [pure_expTheory.Apps_def] \\ metis_tac [])
     \\ rw [] \\ gvs []
     \\ fs [pure_expTheory.Apps_def]
-    \\ rename [‘App (exp_of x5) (Delay (exp_of h5))’]
-    \\ ‘LIST_REL exp_rel [h] [h5]’ by fs []
+    \\ rename [‘App (exp_of x5) (exp_of h5)’]
     \\ qpat_x_assum ‘exp_rel x x5’ assume_tac
-    \\ drule_at (Pos last) exp_rel_App
-    \\ disch_then drule
-    \\ disch_then $ qspec_then ‘ARB’ assume_tac
+    \\ drule exp_rel_App
+    \\ disch_then $ qspecl_then [‘ARB’,‘[h]’,‘[h5]’] mp_tac
+    \\ impl_tac >- (fs [] \\ strip_tac \\ gvs [SF SFY_ss])
+    \\ strip_tac
     \\ first_x_assum $ drule
     \\ fs [GSYM PULL_EXISTS]
     \\ rename [‘LIST_REL _ xs ys’]
@@ -388,23 +498,48 @@ Proof
     \\ disch_then irule
     \\ irule_at Any pure_to_thunk_1ProofTheory.compile_rel_App
     \\ qpat_x_assum ‘to_thunk (exp_of' _) _’ $ irule_at Any
-    \\ qpat_x_assum ‘to_thunk (exp_of' _) _’ $ irule_at Any
     \\ irule_at Any thunk_case_liftProofTheory.compile_rel_App
-    \\ irule_at Any thunk_case_liftProofTheory.compile_rel_Delay
-    \\ qpat_x_assum ‘lift_rel _ _’ $ irule_at Any
-    \\ qpat_x_assum ‘lift_rel _ _’ $ irule_at Any
     \\ irule_at Any thunk_let_forceProofTheory.exp_rel_App
-    \\ irule_at Any thunk_let_forceProofTheory.exp_rel_Delay
-    \\ qpat_x_assum ‘force_rel _ _ _’ $ irule_at Any
-    \\ qpat_x_assum ‘force_rel _ _ _’ $ irule_at Any
     \\ irule_at Any thunk_case_projProofTheory.compile_rel_App
+    \\ irule_at Any thunk_unthunkProofTheory.delay_force_App
+    \\ qpat_x_assum ‘LIST_REL _ _ _’ kall_tac
+    \\ qpat_x_assum ‘(∀c z. h = Var c z ⇒ h5 ≠ Var z) ⇒ _’ mp_tac
+    \\ disch_then (assume_tac o ONCE_REWRITE_RULE [IMP_DISJ_THM])
+    \\ reverse $ gvs []
+    >-
+     (qpat_x_assum ‘to_thunk (exp_of' _) _’ $ irule_at Any
+      \\ qpat_x_assum ‘lift_rel y1 _’ $ irule_at Any
+      \\ qpat_x_assum ‘force_rel NONE y2 _’ $ irule_at Any
+      \\ first_x_assum $ irule_at $ Pos hd
+      \\ irule_at Any thunk_unthunkProofTheory.delay_force_Delay
+      \\ irule_at Any thunk_case_liftProofTheory.compile_rel_Delay
+      \\ first_x_assum $ irule_at $ Pos hd
+      \\ first_x_assum $ irule_at $ Pos hd \\ fs []
+      \\ irule_at Any thunk_case_projProofTheory.compile_rel_Delay
+      \\ first_x_assum $ irule_at $ Pos hd \\ fs []
+      \\ irule_at Any thunk_let_forceProofTheory.exp_rel_Delay
+      \\ fs [cexp_wf_def,SF SFY_ss])
+    \\ first_x_assum $ irule_at $ Pos hd
+    \\ fs [cexp_wf_def,SF SFY_ss,exp_of'_def]
+    \\ qpat_x_assum ‘proj_rel _ y4’ $ irule_at Any
+    \\ qpat_x_assum ‘lift_rel y1 _’ $ irule_at Any \\ gvs []
+    \\ irule_at Any pure_to_thunk_1ProofTheory.compile_rel_Var
+    \\ irule_at Any thunk_case_liftProofTheory.compile_rel_Delay
+    \\ irule_at Any thunk_case_liftProofTheory.compile_rel_Force
+    \\ irule_at Any thunk_case_liftProofTheory.compile_rel_Var
+    \\ irule_at Any thunk_let_forceProofTheory.exp_rel_Delay
+    \\ irule_at Any thunk_let_forceProofTheory.exp_rel_Force
+    \\ irule_at Any thunk_let_forceProofTheory.exp_rel_Var
     \\ irule_at Any thunk_case_projProofTheory.compile_rel_Delay
-    \\ fs [cexp_wf_def])
+    \\ irule_at Any thunk_case_projProofTheory.compile_rel_Force
+    \\ irule_at Any thunk_case_projProofTheory.compile_rel_Var
+    \\ irule_at Any thunk_unthunkProofTheory.delay_force_Delat_Force_Var)
   >~ [‘AtomOp’] >-
    (irule_at Any pure_to_thunk_1ProofTheory.compile_rel_Prim \\ fs []
     \\ irule_at Any thunk_case_liftProofTheory.compile_rel_Prim
     \\ irule_at Any thunk_let_forceProofTheory.exp_rel_Prim
     \\ irule_at Any thunk_case_projProofTheory.compile_rel_Prim \\ fs []
+    \\ irule_at Any thunk_unthunkProofTheory.delay_force_Prim \\ fs []
     \\ pop_assum mp_tac
     \\ pop_assum kall_tac
     \\ pop_assum mp_tac
@@ -420,6 +555,7 @@ Proof
     >- (rpt $ first_assum $ irule_at Any)
     \\ rw []
     \\ irule_at Any pure_to_thunk_1ProofTheory.compile_rel_Lam \\ fs []
+    \\ irule_at Any thunk_unthunkProofTheory.delay_force_Lam \\ fs []
     \\ irule_at Any thunk_case_projProofTheory.compile_rel_Lam \\ fs []
     \\ irule_at Any thunk_case_liftProofTheory.compile_rel_Lam
     \\ irule_at Any thunk_let_forceProofTheory.exp_rel_Lam
@@ -428,6 +564,7 @@ Proof
    (qpat_x_assum ‘_ ≠ []’ kall_tac
     \\ irule_at Any pure_to_thunk_1ProofTheory.compile_rel_Letrec \\ fs []
     \\ irule_at Any thunk_case_projProofTheory.compile_rel_Letrec \\ fs []
+    \\ irule_at Any thunk_unthunkProofTheory.delay_force_Letrec \\ fs []
     \\ irule_at Any thunk_case_liftProofTheory.compile_rel_Letrec
     \\ irule_at Any thunk_let_forceProofTheory.exp_rel_Letrec
     \\ rpt $ first_assum $ irule_at Any
@@ -446,6 +583,7 @@ Proof
     \\ PairCases_on ‘x2’
     \\ gvs []
     \\ irule_at Any thunk_case_liftProofTheory.compile_rel_Delay
+    \\ irule_at Any thunk_unthunkProofTheory.delay_force_Delay
     \\ irule_at Any thunk_case_projProofTheory.compile_rel_Delay
     \\ irule_at Any thunk_let_forceProofTheory.exp_rel_Delay
     \\ rpt $ first_assum $ irule_at Any
@@ -481,11 +619,15 @@ Proof
   \\ impl_keep_tac >-
    (imp_res_tac thunk_case_liftProofTheory.compile_rel_freevars \\ fs [closed_def])
   \\ strip_tac \\ fs []
-  \\ irule_at Any compile_rel_closed \\ fs []
-  \\ first_assum $ irule_at $ Pos hd
-  \\ irule_at Any compile_case_proj_semantics \\ fs []
-  \\ drule exp_rel_NONE_freevars
-  \\ fs [closed_def]
+  \\ drule_at (Pos $ el 2) compile_case_proj_semantics
+  \\ impl_keep_tac
+  >- (drule exp_rel_NONE_freevars \\ fs [closed_def])
+  \\ strip_tac
+  \\ drule thunk_unthunkProofTheory.delay_force_semantics
+  \\ impl_keep_tac
+  >- (imp_res_tac compile_rel_closed \\ gvs [])
+  \\ strip_tac \\ fs []
+  \\ drule_all delay_force_closed \\ fs []
 QED
 
 val _ = export_theory ();
